# baseURI: http://www.w3.org/ns/shacljs
# imports: http://www.w3.org/ns/shacl#

@prefix owl: <http://www.w3.org/2002/07/owl#> .
@prefix rdf: <http://www.w3.org/1999/02/22-rdf-syntax-ns#> .
@prefix rdfs: <http://www.w3.org/2000/01/rdf-schema#> .
@prefix sh: <http://www.w3.org/ns/shacl#> .
@prefix xsd: <http://www.w3.org/2001/XMLSchema#> .

sh:JSConstraint
  rdf:type rdfs:Class ;
  rdfs:label "JavaScript Constraint" ;
  rdfs:subClassOf sh:JSExecutable ;
.
sh:JSConstraint-js
  rdf:type sh:Parameter ;
  sh:path sh:js ;
.
sh:JSConstraintComponent
  rdf:type sh:ConstraintComponent ;
  rdfs:comment "A constraint component with the parameter sh:js linking to a sh:JSConstraint containing a sh:script." ;
  rdfs:label "JavaScript constraint component" ;
  sh:parameter sh:JSConstraint-js ;
.
sh:JSExecutable
  rdf:type rdfs:Class ;
  rdfs:comment "Abstract base class of resources that declare an executable JavaScript." ;
  rdfs:label "JavaScript executable" ;
  rdfs:subClassOf rdfs:Resource ;
.
sh:JSFunction
  rdf:type rdfs:Class ;
  rdfs:comment "A JavaScript function declares a SPARQL function that executes a JavaScript script when called. The arguments of the function become named variables starting with $. For example, the argument ex:test can be accessed by the script via the variable $test. The script must end with a return statement producing a single RDF term, or null." ;
  rdfs:label "JavaScript function"@en ;
  rdfs:subClassOf sh:Function ;
  rdfs:subClassOf sh:JSExecutable ;
.
sh:JSLibrary
  rdf:type rdfs:Class ;
  rdfs:comment "Represents a JavaScript library, typically identified by one or more URLs of files to include." ;
  rdfs:label "JavaScript Library" ;
  rdfs:subClassOf rdfs:Resource ;
.
sh:JSValidator
  rdf:type rdfs:Class ;
  rdfs:comment "A SHACL validator based on JavaScript. This can be used to declare SHACL constraint components that perform JavaScript-based validation when used." ;
  rdfs:label "JavaScript Validator" ;
  rdfs:subClassOf sh:JSExecutable ;
  rdfs:subClassOf sh:Validator ;
.
sh:js
  rdf:type rdf:Property ;
  rdfs:comment "Constraints expressed in JavaScript." ;
  rdfs:label "JavaScript constraint" ;
  rdfs:range sh:JSConstraint ;
.
sh:jsFunctionName
  rdf:type rdf:Property ;
  rdfs:comment "The name of the JavaScript function to execute. Depending on the subclass, this has different execution contracts and expected results." ;
  rdfs:domain sh:JSExecutable ;
  rdfs:label "JavaScript function name" ;
  rdfs:range xsd:string ;
.
sh:jsLibrary
  rdf:type rdf:Property ;
  rdfs:comment "Declares which JavaScript libraries are needed to execute this." ;
  rdfs:domain sh:JSExecutable ;
  rdfs:label "JavaScript library" ;
  rdfs:range sh:JSLibrary ;
.
sh:jsLibraryURL
  rdf:type rdf:Property ;
  rdfs:comment "Declares the URLs of a sh:JSLibrary. This should be the absolute URL of a JavaScript file. Implementations may redirect those to local files." ;
  rdfs:domain sh:JSLibrary ;
  rdfs:label "JavaScript library URL" ;
  rdfs:range xsd:anyURI ;
.
<http://www.w3.org/ns/shacljs>
  rdf:type owl:Ontology ;
  rdfs:comment "Defines the terms used by the SHACL-JS vocabulary." ;
  rdfs:seeAlso <http://w3c.github.io/data-shapes/shacl-js/> ;
  owl:imports sh: ;
  owl:versionInfo "This file contains proposed additions to the SHACL namespace, and may at some stage be added to the main shacl.ttl file." ;
.
